a draft before rejiggering IReads to be recursive

Splinter/plan.i.dfy
@@ -103,6 +103,8 @@ module MsgMapMod {
 }
 
 module JournalMod {
+  import opened Options
+  import opened Sequences
   import opened MsgMapMod
   import opened AllocationMod
 
@@ -113,12 +115,53 @@ module JournalMod {
     messageMap: MsgMap,
     seqStart: nat,  // inclusive
     seqEnd: nat,  // exclusive
-    nextCU: CU   // linked list pointer
+    nextCU: Option<CU>   // linked list pointer
   )
   type JournalChain = seq<JournalRecord>
 
-  predicate ValidJournalChain(journalChain: JournalChain) {
-    false
+  function parse(b: UninterpretedDiskPage) : Option<JournalRecord>
+    // TODO marshalling
+
+  predicate WFChainBasic(journalChain: JournalChain)
+  {
+    && 0 < |journalChain|
+    && Last(journalChain).nextCU.None?
+    && (forall i | 0<=i<|journalChain|-1 :: journalChain[i].nextCU.Some?)
+  }
+
+  predicate {:opaque} WFChainInner(journalChain: JournalChain)
+    requires WFChainBasic(journalChain)
+  {
+    && (forall i | 0<=i<|journalChain|-1 ::
+      journalChain[i].seqStart == journalChain[i+1].seqEnd)
+  }
+
+  predicate WFChain(journalChain: JournalChain)
+  {
+    && WFChainBasic(journalChain)
+    && WFChainInner(journalChain)
+  }
+
+  function CUsForChain(firstCU: CU, journalChain: JournalChain) : (cus: seq<CU>)
+    requires WFChain(journalChain)
+    ensures |cus| == |journalChain|
+  {
+    [firstCU] + seq(|journalChain|-1,
+      i requires 0<=i<|journalChain|-1 => journalChain[i].nextCU.value)
+  }
+
+  predicate RecordOnDisk(dv: DiskView, cu: CU, journalRecord: JournalRecord)
+  {
+    && cu in dv
+    && parse(dv[cu]) == Some(journalRecord)
+  }
+
+  predicate {:opaque} ValidJournalChain(dv: DiskView, firstCU: CU, journalChain: JournalChain) {
+    // Chain is internally consistent
+    && WFChain(journalChain)
+    // ...and it corresponds to stuff in the DiskView starting at firstCU.
+    && var cus := CUsForChain(firstCU, journalChain);
+    && (forall i | 0<=i<|journalChain| :: RecordOnDisk(dv, cus[i], journalChain[i]))
   }
 
   function MessageMaps(journalChain: JournalChain) : seq<MsgMap> {
@@ -127,14 +170,34 @@ module JournalMod {
         => var mm := journalChain[i].messageMap; mm)
   }
 
+  function TheIMChain(dv: DiskView, sb: Superblock) : JournalChain
+    requires exists journalChain :: ValidJournalChain(dv, sb.firstCU, journalChain)
+  {
+    var journalChain :| ValidJournalChain(dv, sb.firstCU, journalChain);
+    journalChain
+  }
+
   function IM(dv: DiskView, sb: Superblock) : MsgMap
   {
-    if (exists journalChain :: ValidJournalChain(journalChain))
+    if (exists journalChain :: ValidJournalChain(dv, sb.firstCU, journalChain))
     then
-      var journalChain :| ValidJournalChain(journalChain);
-      MsgMapMod.ConcatSeq(MessageMaps(journalChain))
+      MsgMapMod.ConcatSeq(MessageMaps(TheIMChain(dv, sb)))
     else
       MsgMapMod.Empty()
+  }
+
+  function {:opaque} IReads(dv: DiskView, firstCU: CU) : set<AU>
+  {
+    if (exists journalChain :: ValidJournalChain(dv, firstCU, journalChain))
+    then
+      var journalChain :| ValidJournalChain(dv, firstCU, journalChain);
+      var cus := CUsForChain(firstCU, journalChain);
+      set i | 0<=i<|cus| :: cus[i].au
+    else
+      // Does this actually work? If there exists no such chain,
+      // did we have to read all the blocks to convince ourselves
+      // of that? Ugh.
+      {}
   }
 
 // Recursive definition, rejected
@@ -143,13 +206,150 @@ module JournalMod {
 //    IMAU(dv, sb.firstCU)
 //  }
 //
-//  function IMAU(dv: DiskView, cu:CU) : Message.MsgMap
+//  function IMAU(dv: DiskView, cu:CU) : Message.MsgMap {
 //    var journalRecord = JournalRecord.I(dv, cu);
 //    suffix := if (firstValidSeq >= journalRecord.lowestSeq)
 //      then MsgMap.Empty()
 //      else IMAU(dv, journalRecord.nextCu);
 //    MsgMap.Concat(journalRecord.msgmap, suffix)
 //  }
+
+  predicate EqualAt(dv0: DiskView, dv1: DiskView, cu: CU)
+    requires cu in dv0
+    requires cu in dv1
+  {
+    dv0[cu]==dv1[cu]
+  }
+
+  predicate Member(dv: DiskView, cu: CU)
+  {
+    cu in dv
+  }
+
+  predicate DiskViewsEquivalentForSet(dv0: DiskView, dv1: DiskView, aus: set<AU>)
+  {
+    && (forall cu:CU :: cu.au in aus ==> Member(dv0, cu))
+    && (forall cu:CU :: cu.au in aus ==> Member(dv1, cu))
+    && (forall cu:CU :: cu.au in aus ==> EqualAt(dv0, dv1, cu))
+  }
+
+  lemma ValidTruncatedChain(dv: DiskView, firstCU: CU, c: JournalChain)
+    requires ValidJournalChain(dv, firstCU, c)
+    requires 1<|c|
+    ensures c[0].nextCU.Some? // boilerplate for next line
+    ensures ValidJournalChain(dv, c[0].nextCU.value, c[1..])
+  {
+    reveal_ValidJournalChain();
+    reveal_WFChainInner();
+  }
+
+  lemma UniqueChain(dv: DiskView, firstCU: CU, c0: JournalChain, c1: JournalChain)
+    requires ValidJournalChain(dv, firstCU, c0)
+    requires ValidJournalChain(dv, firstCU, c1)
+    ensures c0 == c1
+    decreases |c0|
+  {
+    reveal_ValidJournalChain();
+    if |c1|<|c0| {
+      UniqueChain(dv, firstCU, c1, c0);
+    } else {
+      assert c0[0]==c1[0];
+      if 1==|c0| {
+        assert 1==|c1|;
+      } else {
+        ValidTruncatedChain(dv, firstCU, c0);
+        ValidTruncatedChain(dv, firstCU, c1);
+        UniqueChain(dv, c0[0].nextCU.value, c0[1..], c1[1..]);
+      }
+    }
+  }
+
+  lemma CUInIReads(dv: DiskView, firstCU: CU, chain: JournalChain)
+    requires ValidJournalChain(dv, firstCU, chain)
+    ensures firstCU.au in IReads(dv, firstCU)
+  {
+    reveal_IReads();
+    assert ValidJournalChain(dv, firstCU, chain);
+    assert exists journalChain :: ValidJournalChain(dv, firstCU, journalChain);
+    var journalChain :| ValidJournalChain(dv, firstCU, journalChain);
+    UniqueChain(dv, firstCU, chain, journalChain);
+    assert chain == journalChain;
+    assert firstCU.au in IReads(dv, firstCU);
+  }
+
+  lemma FrameOneChain(dv0: DiskView, dv1: DiskView, firstCU: CU, journalChain: JournalChain)
+    requires ValidJournalChain(dv0, firstCU, journalChain)
+    requires DiskViewsEquivalentForSet(dv0, dv1, IReads(dv0, firstCU))
+    ensures ValidJournalChain(dv1, firstCU, journalChain)
+    decreases |journalChain|
+  {
+    reveal_ValidJournalChain();
+    if |journalChain|==1 {
+      assert WFChain(journalChain);
+      // ...and it corresponds to stuff in the DiskView starting at firstCU.
+      var cus := CUsForChain(firstCU, journalChain);
+      forall i | 0<=i<|journalChain|
+        ensures RecordOnDisk(dv1, cus[i], journalChain[i])
+      {
+        assert i == 0;
+        assert cus[i] == firstCU;
+        assert RecordOnDisk(dv0, firstCU, journalChain[i]);
+        CUInIReads(dv0, firstCU, journalChain);
+        assert EqualAt(dv0, dv1, firstCU);
+        assert RecordOnDisk(dv1, firstCU, journalChain[i]);
+        assert RecordOnDisk(dv1, cus[i], journalChain[i]);
+      }
+      assert ValidJournalChain(dv1, firstCU, journalChain);
+    } else {
+      var secondCU := journalChain[0].nextCU.value;
+      ValidTruncatedChain(dv0, firstCU, journalChain);
+      assert IReads(dv0, secondCU) <= IReads(dv0, firstCU);
+      assert DiskViewsEquivalentForSet(dv0, dv1, IReads(dv0, secondCU));
+      FrameOneChain(dv0, dv1, secondCU, journalChain[1..]);
+
+      // Sequence math to enjoy results of recursion
+      var cus := CUsForChain(firstCU, journalChain);
+      var cus1 := CUsForChain(secondCU, journalChain[1..]);
+      forall i | 0<=i<|journalChain|
+        ensures RecordOnDisk(dv1, cus[i], journalChain[i])
+      {
+        //assert cus[i] in IReads(dv0, firstCU);
+        if i==0 {
+          assert RecordOnDisk(dv1, cus[i], journalChain[i]);
+        } else {
+          assert RecordOnDisk(dv1, cus1[i-1], journalChain[1..][i-1]);
+          assert RecordOnDisk(dv1, cus[i], journalChain[i]);
+        }
+      }
+
+      assert ValidJournalChain(dv1, firstCU, journalChain);
+    }
+  }
+
+
+  lemma Framing(sb:Superblock, dv0: DiskView, dv1: DiskView)
+    requires DiskViewsEquivalentForSet(dv0, dv1, IReads(dv0, sb.firstCU))
+    ensures IM(dv0, sb) == IM(dv1, sb)
+  {
+    var le0 := exists journalChain :: ValidJournalChain(dv0, sb.firstCU, journalChain);
+    var le1 := exists journalChain :: ValidJournalChain(dv1, sb.firstCU, journalChain);
+    if le0 && le1 {
+      var journalChain0 := TheIMChain(dv0, sb);
+      var journalChain1 := TheIMChain(dv1, sb);
+      FrameOneChain(dv0, dv1, sb.firstCU, journalChain0);
+      UniqueChain(dv1, sb.firstCU, journalChain0, journalChain1);
+      assert journalChain0 == journalChain1;
+      calc {
+        IM(dv0, sb);
+        MsgMapMod.ConcatSeq(MessageMaps(journalChain0));
+        MsgMapMod.ConcatSeq(MessageMaps(journalChain1));
+        IM(dv1, sb);
+      }
+    } else {
+      assume false;
+      assert IM(dv0, sb) == IM(dv1, sb);
+    }
+  }
 }
 
 module MarshalledSnapshot {
@@ -205,6 +405,7 @@ module IndirectionTableMod refines MarshalledSnapshot {
 }
 
 module BetreeMod {
+  import opened Options
   import opened MessageMod
   import opened AllocationMod
   import opened MsgSeqMod
@@ -213,16 +414,16 @@ module BetreeMod {
 
   datatype Superblock = Superblock(itbl: IndirectionTableMod.Superblock, rootIdx: IndirectionTableMod.IndirectionTable)
 
-  datatype LookupRecord = LookupRecord()
+  datatype LookupRecord = LookupRecord(
+    cu: CU
+  )
   type Lookup = seq<LookupRecord>
 
   function LookupToMsgSeq(lookup: Lookup) : MsgSeq
     // TODO body
 
   predicate ValidLookup(dv: DiskView, itbl: IndirectionTable, key: Key, lookup: Lookup)
-  {
-    false // TODO
-  }
+    // TODO
 
   function IMKey(dv: DiskView, sb: Superblock, key: Key) : MsgSeq
   {
@@ -240,6 +441,55 @@ module BetreeMod {
   function IM(dv: DiskView, sb: Superblock) : MsgMap
   {
     imap key | key in AllKeys() :: IMKey(dv, sb, key)
+  }
+
+  function IReadsKey(dv: DiskView, itbl: Option<IndirectionTable>, key: Key) : set<AU> {
+    
+    if
+      && itbl.Some?
+      && exists lookup :: ValidLookup(dv, itbl.value, key, lookup)
+    then
+      var lookup :| ValidLookup(dv, itbl.value, key, lookup);
+      set i | 0<=i<|lookup| :: var lr:LookupRecord := lookup[i]; lr.cu.au
+    else
+      {}
+  }
+
+  function IReads(dv: DiskView, sb: Superblock) : set<AU> {
+    var itbl := IndirectionTableMod.I(dv, sb.itbl);
+    set au:AU |
+      && au < AUSizeInBlocks()
+      && exists key :: au in IReadsKey(dv, itbl, key)
+  }
+
+  lemma Framing(sb:Superblock, dv0: DiskView, dv1: DiskView)
+    requires forall cu:CU :: cu.au in IReads(dv0, sb) ==>
+      && cu in dv0
+      && cu in dv1
+      && dv0[cu]==dv1[cu]
+    ensures IM(dv0, sb) == IM(dv1, sb)
+  {
+    // TODO I'm surprised this proof passes easily.
+    forall key | key in AllKeys()
+      ensures IMKey(dv0, sb, key) == IMKey(dv1, sb, key)
+    {
+      var itbl0 := IndirectionTableMod.I(dv0, sb.itbl);
+      var itbl1 := IndirectionTableMod.I(dv1, sb.itbl);
+      if itbl0.Some? && itbl1.Some?
+      {
+        var le0 := exists lookup0 :: ValidLookup(dv0, itbl0.value, key, lookup0);
+        var le1 := exists lookup1 :: ValidLookup(dv1, itbl1.value, key, lookup1);
+        if le0 {
+          var lookup0 :| ValidLookup(dv0, itbl0.value, key, lookup0);
+          assert ValidLookup(dv1, itbl1.value, key, lookup0);
+        }
+        if le1 {
+          var lookup1 :| ValidLookup(dv1, itbl1.value, key, lookup1);
+          assert ValidLookup(dv0, itbl1.value, key, lookup1);
+        }
+        assert le0 == le1;
+      }
+    }
   }
 }
 
@@ -281,6 +531,11 @@ module System {
     else
       None  // silly expression: DV has holes in it
   }
+
+  function ISuperblockReads(dv: DiskView) : set<AU>
+  {
+    {0}
+  }
  
   // IM == Interpret as MsgSeq
   // Oh man we're gonna have a family of IReads predicates that capture the
@@ -295,7 +550,58 @@ module System {
       MsgMapMod.Empty()
   }
 
+  function IMReads(dv: DiskView) : set<AU> {
+      {}
+      /*
+    var sb := ISuperblock(dv);
+    if sb.Some?
+    then
+      JournalMod.IReads(dv, sb.value.journal) + BetreeMod.IReads(dv, sb.value.betree)
+    else
+      set{}
+      */
+  }
+
   function I(dv: DiskView) : imap<Key, Value> {
     MsgMapMod.I(IM(dv))
   }
+
+  function IReads(dv: DiskView) : set<AU> {
+    IMReads(dv)
+  }
+
+  lemma Framing(dv0: DiskView, dv1: DiskView)
+  /*
+    requires forall cu:CU :: cu.au in IReads(dv0) ==>
+      && cu in dv0
+      && cu in dv1
+      && dv0[cu]==dv1[cu]
+      */
+    ensures I(dv0) == I(dv1)
+  {
+    //assert forall k :: k !in I(dv0);
+    assert forall k :: I(dv0)[k] == I(dv1)[k];
+  }
 }
+
+/*
+Okay, so the magic is going to be that
+- most of the time when we change a block in RAM we'll prove that it's
+  not in use in any other view
+  - that'll depend on an invariant between the allocation table
+    and the IReads functions
+  - And we'll need a proof that, if IReads doesn't change, I doesn't
+    change, of course.
+- when we write a non-superblock back to disk, we inherit that no-change
+  property; the persistent view doesn't change because the thing
+  we wrote back was dirty and hence outside of the IReads of the
+  persistent view.
+- when we update the superblock, we're creating a frozen view.
+- when we write a superblock back, it's easy again, because the persistent
+  view just vanishes, replaced by the frozen view.
+  The vanishing old persistent view implicitly creates some free nodes,
+  which can be detected because the available nodes are computed at
+  runtime by reading the active AllocationTables, and one just became
+  empty.
+  (that is, the union of allocationTables will cover the IReads sets.)
+*/
